code/bexpr.thy
@@ -8,7 +8,7 @@ datatype 'b bexpr =
     | BAnd "'b bexpr" "'b bexpr"
     | BLeq "'b aexpr" "'b aexpr"
 
-inductive eval_bexpr :: "int bexpr \<Rightarrow> int state \<Rightarrow> bool behaviour \<Rightarrow> bool" where
+inductive eval_bexpr :: " 'a bexpr \<Rightarrow> 'a state \<Rightarrow> bool behaviour \<Rightarrow> bool" where
 EBCst : "eval_bexpr (BCst b) s (Enormal b)"
 | EBNot : "eval_bexpr b s (Enormal b') \<Longrightarrow>
            eval_bexpr (BNot b) s (Enormal (\<not> b'))"
@@ -16,8 +16,7 @@ EBCst : "eval_bexpr (BCst b) s (Enormal b)"
                eval_bexpr (BNot b) s Eunbound"
 | EBAnd : "eval_bexpr b1 s (Enormal b1') \<Longrightarrow>
            eval_bexpr b2 s (Enormal b2') \<Longrightarrow>
-           b1' \<and> b2' = b3 \<Longrightarrow>
-           eval_bexpr (BAnd b1 b2) s (Enormal b3)"
+           eval_bexpr (BAnd b1 b2) s (Enormal (b1' \<and> b2'))"
 | EBAnd_err1 : "eval_bexpr b1 s Eunbound \<Longrightarrow>
                 eval_bexpr (BAnd b1 b2) s Eunbound"
 | EBAnd_err2 : "eval_bexpr b1 s (Enormal b1') \<Longrightarrow>
@@ -32,31 +31,30 @@ EBCst : "eval_bexpr (BCst b) s (Enormal b)"
                 eval_aexpr a2 s Eunbound \<Longrightarrow>
                 eval_bexpr (BLeq a1 a2) s Eunbound"
 
+inductive_cases eval_bexpr_BCstE[elim!]: "eval_bexpr (BCst n) s b"
+            and eval_bexpr_BNotE[elim!]: "eval_bexpr (BNot b1) s b"
+            and eval_bexpr_BAndE[elim!]: "eval_bexpr (BAnd b1 b2) s b"
+            and eval_bexpr_BLeqE[elim!]: "eval_bexpr (BLeq a1 a2) s b"
 
-inductive_cases eval_aexpr_BCstE[elim!]: "eval_aexpr (Cst n) s b"
-            and eval_aexpr_BNotE[elim!]: "eval_aexpr (Var n) s b"
-            and eval_aexpr_BAndE[elim!]: "eval_aexpr (BinOp a1 op a2) s b"
-            and eval_aexpr_BAndE[elim!]: "eval_aexpr (BinOp a1 op a2) s b"
-
-
+thm eval_bexpr_BLeqE
 
 lemma eval_bexpr_fun :
  "\<lbrakk>eval_bexpr b s b1; eval_bexpr b s b2\<rbrakk> \<Longrightarrow> b1 = b2"
-proof(induction b arbitrary: b1 s b2)
-  case (BCst x)
-  then show ?case by(auto intro: eval_bexpr.cases)
+proof(induction arbitrary: b2 rule: eval_bexpr.induct)
+  case (EBLeq a1 s n1 a2 n2)
+  then show ?case 
+    using eval_bexpr_BLeqE eval_aexpr_fun
+    by (metis behaviour.inject behaviour.simps(3))
 next
-  case (BNot b)
-  then show ?case using eval_bexpr.cases
-(*next
-  case (BAnd b1 b2)
-  then show ?case sorry*)
+  case (EBLeq_err1 a1 s a2)
+  then show ?case 
+    using eval_aexpr_fun by blast
 next
-  case (BLeq x1a x2a)
-  then show ?case using
-    by (smt (verit) behaviour.distinct(1) behaviour.inject bexpr.distinct(5) 
-        bexpr.distinct(9) bexpr.inject(4) eval_aexpr_fun_version2 eval_bexpr.cases)
-qed
+  case (EBLeq_err2 a1 s n1 a2)
+  then show ?case
+    using eval_aexpr_fun by blast
+next
+qed auto
 
 end
 
