code/stmt.thy
@@ -1,0 +1,184 @@
+theory stmt
+  imports formula
+begin
+
+datatype 'a stmt =
+  SSkip
+  | SSeq "'a stmt" "'a stmt" 
+  | Sassign 'a "'a aexpr"
+  | Sassert "'a formula"
+  | SIf "'a bexpr" "'a stmt" "'a stmt"
+  | Swhile "'a bexpr" "'a formula" "'a stmt"
+
+fun subst_aexpr :: "int aexpr \<Rightarrow> int \<Rightarrow> int \<Rightarrow> int aexpr" where
+  "subst_aexpr (Cst n) x v = (Cst n)"
+| "subst_aexpr (Var y) x v = (if x = y then Var v else Var y)"
+| "subst_aexpr (BinOp a1 op a2) x v = BinOp (subst_aexpr a1 x v) op (subst_aexpr a2 x v)"
+
+fun subst_bexpr :: "int bexpr \<Rightarrow> int \<Rightarrow> int \<Rightarrow> int bexpr" where
+  "subst_bexpr (BCst b) x v = BCst b"
+| "subst_bexpr (BLeq a1 a2) x v = BLeq (subst_aexpr a1 x v) (subst_aexpr a2 x v)"
+| "subst_bexpr (BAnd b1 b2) x v = BAnd (subst_bexpr b1 x v) (subst_bexpr b2 x v)"
+| "subst_bexpr (BNot b) x v = BNot (subst_bexpr b x v)"
+
+fun subst_formula :: "int formula \<Rightarrow> int \<Rightarrow> int \<Rightarrow> int formula" where
+  "subst_formula (FTerm b) x v = FTerm (subst_bexpr b x v)"
+| "subst_formula (FAnd f1 f2) x v = FAnd (subst_formula f1 x v) (subst_formula f2 x v)"
+| "subst_formula (FNot f) x v = FNot (subst_formula f x v)"
+| "subst_formula (FImp f1 f2) x v = FImp (subst_formula f1 x v) (subst_formula f2 x v)"
+| "subst_formula (FAll y f) x v = FAll y (subst_formula f x v)"
+
+fun abstract_effects :: "int stmt \<Rightarrow> int formula \<Rightarrow> int formula" where
+   "abstract_effects SSkip f = f"
+ | "abstract_effects (Sassert _) f = f"
+ | "abstract_effects (SSeq s1 s2) f = abstract_effects s2 (abstract_effects s1 f)"
+ | "abstract_effects (SIf _ s1 s2) f = abstract_effects s2 (abstract_effects s1 f)"
+ | "abstract_effects (Sassign x _) f = (let v = fresh_from f in
+                                        let f' = subst_formula f x v in
+                                        FAll v f')" 
+ | "abstract_effects (Swhile _ _ s) f = abstract_effects s f"
+
+definition formula_equiv_sem :: "'a formula \<Rightarrow> 'a formula \<Rightarrow> bool" (infixl "\<approx>" 40) where
+  "f1 \<approx> f2 \<longleftrightarrow> (\<forall>st. eval_formula f1 st = eval_formula f2 st)"
+
+
+(*lemma subst_not_occur : "x \<notin> vars_in_formula f \<Longrightarrow> eval_formula (FAll *)
+lemma fall_elim : 
+  assumes "x \<notin> fv_formula f"
+  and "eval_formula (FAll v f) st"
+  shows "eval_formula (subst_formula f v x) st"
+  using assms oops
+
+lemma subst_then_no_vars : "x \<noteq> v \<Longrightarrow> f' = (subst_formula f x v) \<Longrightarrow> x \<notin> fv_formula f'"
+  oops
+
+lemma abstract_effects_specialize : "eval_formula (abstract_effects s f) st \<Longrightarrow> eval_formula f st"
+proof(induction s arbitrary: f st)
+  case SSkip
+  then show ?case by simp
+next
+  case (SSeq s1 s2)
+  then show ?case
+    by (metis abstract_effects.simps(3))
+next
+  case (Sassign x a)
+  then show ?case apply(auto simp: Let_def) sorry
+next
+  case (Sassert x)
+  then show ?case by simp
+next
+  case (SIf x1 s1 s2)
+  then show ?case
+    by (metis abstract_effects.simps(4))
+next
+  case (Swhile x1 x2 s)
+  then show ?case
+    by (metis abstract_effects.simps(6))
+qed
+
+lemma abstract_effects_distrib_conj :
+  "(eval_formula (abstract_effects s p) st \<and> eval_formula (abstract_effects s q) st) \<Longrightarrow>
+  eval_formula (abstract_effects s (FAnd p q)) st"
+proof(induction s arbitrary: p q)
+  case (SSeq s1 s2)
+  then show ?case apply(simp) sorry
+next
+  case (Sassign x1 x2)
+  then show ?case sorry
+next
+  case (SIf x1 s1 s2)
+  then show ?case sorry
+qed simp_all
+
+definition valid_formula :: "'a formula \<Rightarrow> bool" where
+  "valid_formula f \<longleftrightarrow> (\<forall> st. eval_formula f st)"
+
+lemma abstract_effects_monotonic :
+  "valid_formula (FImp p q) \<Longrightarrow>
+   eval_formula (abstract_effects s p) st \<Longrightarrow>
+   eval_formula (abstract_effects s q) st"
+proof(induction s arbitrary: p q st)
+  case (SSeq s1 s2)
+  then show ?case apply(simp add: valid_formula_def) by blast
+next
+  case (Sassign x1 x2)
+  then show ?case apply(simp add: valid_formula_def Let_def) sorry
+next
+  case (SIf x1 s1 s2)
+  then show ?case apply(auto simp: valid_formula_def) by blast
+qed (auto simp: valid_formula_def)
+
+fun wp :: "int stmt \<Rightarrow> int formula \<Rightarrow> int formula" where
+  "wp SSkip q = q"
+| "wp (SSeq s1 s2) q = wp s1 (wp s2 q)"
+| "wp (Sassert p) q = FAnd p (FImp p q)"
+| "wp (Sassign x e) q = (let y = fresh_from q in
+                        FAll y (FImp (FAnd (FTerm (BLeq (Var y) e))
+                                           (FTerm (BLeq e (Var y))))
+                               (subst_formula q x y)))"
+| "wp (SIf b s1 s2) q = FAnd (FImp (FTerm b) (wp s1 q))
+                             (FImp (FNot (FTerm b)) (wp s2 q))"
+| "wp (Swhile cond invariant body) q =
+   FAnd invariant
+        (abstract_effects body
+        (FAnd (FImp (FAnd (FTerm cond) invariant) (wp body invariant))
+              (FImp (FAnd (FNot (FTerm cond)) invariant) q)))"
+
+lemma abstract_effect_writes :
+  "eval_formula (abstract_effects s q) st \<Longrightarrow>
+   eval_formula (wp s (abstract_effects s q)) st"
+proof(induction s arbitrary: q)
+  case SSkip
+  then show ?case by simp
+next
+  case (SSeq s1 s2)
+  then show ?case sorry
+next
+  case (Sassign x1 x2)
+  then show ?case sorry
+next
+  case (Sassert x)
+  then show ?case sorry
+next
+  case (SIf x1 s1 s2)
+  then show ?case sorry
+next
+  case (Swhile x1 x2 s)
+  then show ?case sorry
+qed
+
+
+lemma monotonicity : "valid_formula (FImp p q) \<Longrightarrow>
+  valid_formula (FImp (wp s p) (wp s q))"
+proof(induction s arbitrary: p q)
+  case (SSeq s1 s2)
+  then show ?case
+    using wp.simps(2) by presburger
+next
+  case (Sassign x1 x2)
+  then show ?case
+    by (metis abstract_effect_writes abstract_effects.simps(2) eval_formula.simps(2) valid_formula_def wp.simps(3))
+next
+  case (Swhile x1 x2 s)
+  then show ?case
+    by (metis abstract_effect_writes abstract_effects.simps(2) eval_formula.simps(2) valid_formula_def wp.simps(3))
+qed (simp_all add: valid_formula_def)
+
+lemma distrib_conj : 
+  "eval_formula (wp s p) st \<and> eval_formula (wp s q) st \<Longrightarrow>
+   eval_formula (wp s (FAnd p q)) st"
+proof(induction s arbitrary: p q st)
+  case (SSeq s1 s2)
+  then show ?case
+    by (metis abstract_effect_writes abstract_effects.simps(2) eval_formula.simps(2) wp.simps(3))
+next
+  case (Sassign x1 x2)
+  then show ?case
+    by (metis abstract_effect_writes abstract_effects.simps(2) eval_formula.simps(2) wp.simps(3))
+next
+  case (Swhile x1 x2 s)
+  then show ?case
+    by (metis abstract_effect_writes abstract_effects.simps(2) eval_formula.simps(2) wp.simps(3))
+qed simp_all
+
+end
